[minor] Make Determinism compile faster.
Try to avoid need for inversion as much as possible by adding explicit
equalities to the step relation.

pico-ifc-coq/dyn_allocation/ConcreteMachine.v
@@ -36,181 +36,229 @@ Definition c_alloc (p:privilege) (size:Z) (a:Atom) (m:memory) :=
 (** Concrete machine transition relation.
     Each instructions has 3 semantic rules: (user mode - succ) (user mode - faulting) (kernel mode) *)
 
-Inductive cstep : CS -> CEvent+τ -> CS -> Prop := 
+Inductive cstep (cs1 : CS) (ca : CEvent+τ) (cs2 : CS) : Prop :=
 | cstep_nop : forall m fh i s pcv pcl rl rpcl,
     forall (INST: i @ pcv # Noop)
            (CHIT: cache_hit_mem m (opCodeToZ OpNoop) (__,__,__) pcl)
-           (CREAD: cache_hit_read_mem m rl rpcl),
-    cstep (CState m fh i s (pcv,pcl) false)
-          Silent (CState m fh i s (pcv+1,rpcl) false)
+           (CREAD: cache_hit_read_mem m rl rpcl)
+           (CS1: cs1 = CState m fh i s (pcv,pcl) false)
+           (CA: ca = Silent)
+           (CS2: cs2 = CState m fh i s (pcv+1,rpcl) false),
+    cstep cs1 ca cs2
 
 | cstep_nop_f : forall c' m fh i s pcv pcl m',
    forall (INST: i @ pcv # Noop)
           (CMISS: ~ cache_hit_mem m (opCodeToZ OpNoop) (__,__,__) pcl)
           (CUPD: c' = build_cache (opCodeToZ OpNoop) (__,__,__)  pcl)
-          (CUPDGET: cupd m c' = Some m'),
-    cstep (CState m fh i s (pcv,pcl) false) 
-          Silent (CState m' fh i ((fh_ret pcv pcl)::s) fh_start true)
+          (CUPDGET: cupd m c' = Some m')
+          (CS1: cs1 = CState m fh i s (pcv,pcl) false)
+          (CA: ca = Silent)
+          (CS2: cs2 = CState m' fh i ((fh_ret pcv pcl)::s) fh_start true),
+    cstep cs1 ca cs2
 
 | cstep_nop_p : forall m fh i s pcv pcl,
-    fh @ pcv # Noop ->
-    cstep (CState m fh i s (pcv,pcl) true) Silent (CState m fh i s (pcv+1,handlerTag) true)
+    forall (INST: fh @ pcv # Noop)
+           (CS1: cs1 = CState m fh i s (pcv,pcl) true)
+           (CA: ca = Silent)
+           (CS2: cs2 = CState m fh i s (pcv+1,handlerTag) true),
+    cstep cs1 ca cs2
 
 | cstep_add: forall fh m i s rpcl pcv pcl rl x1v x1l x2v x2l v,
    forall(INST: i @ pcv # Add)
          (CHIT: cache_hit_mem m (opCodeToZ OpAdd) (x1l, x2l, __) pcl)
          (CREAD: cache_hit_read_mem m rl rpcl)
-         (ADD: add x1v x2v = Some v),
-     cstep (CState m fh i ((x1v,x1l):::(x2v,x2l):::s) (pcv,pcl)    false)  
-           Silent (CState m fh i          ((v,rl):::s) (pcv+1,rpcl) false)
+         (ADD: add x1v x2v = Some v)
+         (CS1: cs1 = CState m fh i ((x1v,x1l):::(x2v,x2l):::s) (pcv,pcl) false)
+         (CA: ca = Silent)
+         (CS2: cs2 = CState m fh i ((v,rl):::s) (pcv+1,rpcl) false),
+     cstep cs1 ca cs2
 
 | cstep_add_f: forall c' fh m i s pcv pcl x1v x1l x2v x2l m',
    forall(INST: i @ pcv # Add)
          (CMISS: ~ cache_hit_mem m (opCodeToZ OpAdd) (x1l, x2l, __) pcl)
          (CUPD: c' = build_cache (opCodeToZ OpAdd) (x1l,x2l,__)  pcl)
-         (CUPDGET: cupd m c' = Some m'),
-     cstep (CState m fh i ((x1v,x1l):::(x2v,x2l):::s) (pcv,pcl)    false)  
-           Silent (CState m' fh i ((fh_ret pcv pcl)::(x1v,x1l):::(x2v,x2l):::s) fh_start true)
+         (CUPDGET: cupd m c' = Some m')
+         (CS1: cs1 = CState m fh i ((x1v,x1l):::(x2v,x2l):::s) (pcv,pcl) false)
+         (CA: ca = Silent)
+         (CS2: cs2 = CState m' fh i ((fh_ret pcv pcl)::(x1v,x1l):::(x2v,x2l):::s) fh_start true),
+     cstep cs1 ca cs2
 
-| cstep_add_p: forall m fh i s pcv pcl x1v x1l x2v x2l v, 
-    fh @ pcv # Add ->
-    add x1v x2v = Some v ->
-    cstep (CState m fh i ((x1v,x1l):::(x2v,x2l):::s) (pcv,pcl) true)  
-          Silent (CState m fh i ((v,handlerTag):::s) (pcv+1,handlerTag) true)
+| cstep_add_p: forall m fh i s pcv pcl x1v x1l x2v x2l v,
+    forall (INST: fh @ pcv # Add)
+           (ADD: add x1v x2v = Some v)
+           (CS1: cs1 = CState m fh i ((x1v,x1l):::(x2v,x2l):::s) (pcv,pcl) true)
+           (CA: ca = Silent)
+           (CS2: cs2 = CState m fh i ((v,handlerTag):::s) (pcv+1,handlerTag) true),
+    cstep cs1 ca cs2
 
 | cstep_sub: forall fh m i s rpcl pcv  pcl rl x1v x1l x2v x2l v,
    forall(INST: i @ pcv # Sub)
          (CHIT: cache_hit_mem m (opCodeToZ OpSub) (x1l, x2l, __) pcl)
          (CREAD: cache_hit_read_mem m rl rpcl)
-         (SUB: sub x1v x2v = Some v),
-     cstep (CState m fh i ((x1v,x1l):::(x2v,x2l):::s) (pcv,pcl)    false)  
-           Silent (CState m fh i          ((v,rl):::s) (pcv+1,rpcl) false)
+         (SUB: sub x1v x2v = Some v)
+         (CS1: cs1 = CState m fh i ((x1v,x1l):::(x2v,x2l):::s) (pcv,pcl) false)
+         (CA: ca = Silent)
+         (CS2: cs2 = CState m fh i ((v,rl):::s) (pcv+1,rpcl) false),
+     cstep cs1 ca cs2
 
 | cstep_sub_f: forall c' fh m i s pcv pcl x1v x1l x2v x2l m',
    forall(INST: i @ pcv # Sub)
          (CMISS: ~ cache_hit_mem m (opCodeToZ OpSub) (x1l, x2l, __) pcl)
          (CUPD: c' = build_cache (opCodeToZ OpSub) (x1l,x2l,__)  pcl)
-         (CUPDGET: cupd m c' = Some m'),
-     cstep (CState m fh i ((x1v,x1l):::(x2v,x2l):::s) (pcv,pcl)    false)  
-           Silent (CState m' fh i ((fh_ret pcv pcl)::(x1v,x1l):::(x2v,x2l):::s) fh_start true)
+         (CUPDGET: cupd m c' = Some m')
+         (CS1: cs1 = CState m fh i ((x1v,x1l):::(x2v,x2l):::s) (pcv,pcl) false)
+         (CA: ca = Silent)
+         (CS2: cs2 = CState m' fh i ((fh_ret pcv pcl)::(x1v,x1l):::(x2v,x2l):::s) fh_start true),
+     cstep cs1 ca cs2
 
-| cstep_sub_p: forall m fh i s pcv pcl x1v x1l x2v x2l v, 
-    fh @ pcv # Sub ->
-    sub x1v x2v = Some v ->
-    cstep (CState m fh i ((x1v,x1l):::(x2v,x2l):::s) (pcv,pcl) true) 
-          Silent (CState m fh i ((v,handlerTag):::s) (pcv+1,handlerTag) true)
+| cstep_sub_p: forall m fh i s pcv pcl x1v x1l x2v x2l v,
+    forall (INST: fh @ pcv # Sub)
+           (SUB: sub x1v x2v = Some v)
+           (CS1: cs1 = CState m fh i ((x1v,x1l):::(x2v,x2l):::s) (pcv,pcl) true)
+           (CA: ca = Silent)
+           (CS2: cs2 = CState m fh i ((v,handlerTag):::s) (pcv+1,handlerTag) true),
+    cstep cs1 ca cs2
 
 | cstep_eq: forall fh m i s rpcl pcv  pcl rl x1v x1l x2v x2l,
    forall(INST: i @ pcv # Eq)
          (CHIT: cache_hit_mem m (opCodeToZ OpEq) (x1l, x2l, __) pcl)
-         (CREAD: cache_hit_read_mem m rl rpcl),
-     cstep (CState m fh i ((x1v,x1l):::(x2v,x2l):::s) (pcv,pcl)    false)
-           Silent (CState m fh i          ((val_eq x1v x2v,rl):::s) (pcv+1,rpcl) false)
+         (CREAD: cache_hit_read_mem m rl rpcl)
+         (CS1: cs1 = CState m fh i ((x1v,x1l):::(x2v,x2l):::s) (pcv,pcl)    false)
+         (CA: ca = Silent)
+         (CS2: cs2 = CState m fh i          ((val_eq x1v x2v,rl):::s) (pcv+1,rpcl) false),
+     cstep cs1 ca cs2
 
 | cstep_eq_f: forall c' fh m i s pcv pcl x1v x1l x2v x2l m',
    forall(INST: i @ pcv # Eq)
          (CMISS: ~ cache_hit_mem m (opCodeToZ OpEq) (x1l, x2l, __) pcl)
          (CUPD: c' = build_cache (opCodeToZ OpEq) (x1l,x2l,__)  pcl)
-         (CUPDGET: cupd m c' = Some m'),
-     cstep (CState m fh i ((x1v,x1l):::(x2v,x2l):::s) (pcv,pcl)    false)
-           Silent (CState m' fh i ((fh_ret pcv pcl)::(x1v,x1l):::(x2v,x2l):::s) fh_start true)
+         (CUPDGET: cupd m c' = Some m')
+         (CS1: cs1 = CState m fh i ((x1v,x1l):::(x2v,x2l):::s) (pcv,pcl)    false)
+         (CA: ca = Silent)
+         (CS2: cs2 = CState m' fh i ((fh_ret pcv pcl)::(x1v,x1l):::(x2v,x2l):::s) fh_start true),
+     cstep cs1 ca cs2
 
 | cstep_eq_p: forall m fh i s pcv pcl x1v x1l x2v x2l,
-    fh @ pcv # Eq ->
-    cstep (CState m fh i ((x1v,x1l):::(x2v,x2l):::s) (pcv,pcl) true)
-          Silent (CState m fh i ((val_eq x1v x2v,handlerTag):::s) (pcv+1,handlerTag) true)
+    forall (INST: fh @ pcv # Eq)
+           (CS1: cs1 = CState m fh i ((x1v,x1l):::(x2v,x2l):::s) (pcv,pcl) true)
+           (CA: ca = Silent)
+           (CS2: cs2 = CState m fh i ((val_eq x1v x2v,handlerTag):::s) (pcv+1,handlerTag) true),
+    cstep cs1 ca cs2
 
 | cstep_dup_p: forall m fh i s pcv pcl n x,
-    fh @ pcv # Dup n ->
-    index_list n s = Some x ->
-    cstep (CState m fh i s (pcv,pcl) true)
-          Silent (CState m fh i (x::s) (pcv+1,handlerTag) true)
+    forall (INST: fh @ pcv # Dup n)
+           (DUP: index_list n s = Some x)
+           (CS1: cs1 = CState m fh i s (pcv,pcl) true)
+           (CA: ca = Silent)
+           (CS2: cs2 = CState m fh i (x::s) (pcv+1,handlerTag) true),
+    cstep cs1 ca cs2
 
 | cstep_swap_p: forall m fh i y s pcv pcl n x s',
-    fh @pcv # Swap n -> 
-    index_list n (y::s) = Some x ->
-    update_list n y (x::s) = Some s' ->
-    cstep (CState m fh i (y::s) (pcv,pcl) true)
-          Silent (CState m fh i s' (pcv+1,handlerTag) true)
+    forall (INST: fh @pcv # Swap n)
+           (IDX: index_list n (y::s) = Some x)
+           (UPD: update_list n y (x::s) = Some s')
+           (CS1: cs1 = CState m fh i (y::s) (pcv,pcl) true)
+           (CA: ca = Silent)
+           (CS2: cs2 = CState m fh i s' (pcv+1,handlerTag) true),
+    cstep cs1 ca cs2
 
 | cstep_push: forall fh m i s rpcl pcv pcl rl cv,
    forall(INST: i @ pcv # Push cv)
          (CHIT: cache_hit_mem m (opCodeToZ OpPush) (__ , __, __) pcl)
-         (CREAD: cache_hit_read_mem m rl rpcl),
-     cstep (CState m fh i s (pcv,pcl)   false)
-           Silent (CState m fh i ((Vint cv,rl):::s) (pcv+1,rpcl) false)
+         (CREAD: cache_hit_read_mem m rl rpcl)
+         (CS1: cs1 = CState m fh i s (pcv,pcl)   false)
+         (CA: ca = Silent)
+         (CS2: cs2 = CState m fh i ((Vint cv,rl):::s) (pcv+1,rpcl) false),
+     cstep cs1 ca cs2
 
 | cstep_push_f: forall c' fh m i s pcv pcl cv m',
    forall(INST : i @ pcv # Push cv)
          (CMISS: ~ cache_hit_mem m (opCodeToZ OpPush) (__,__,__) pcl)
          (CUPD : c' = build_cache (opCodeToZ OpPush) (__,__,__) pcl)
-         (CUPDGET : cupd m c' = Some m'),
-     cstep (CState m fh i s (pcv,pcl) false)  
-           Silent (CState m' fh i ((fh_ret pcv pcl)::s) fh_start true)
+         (CUPDGET : cupd m c' = Some m')
+         (CS1: cs1 = CState m fh i s (pcv,pcl) false)
+         (CA: ca = Silent)
+         (CS2: cs2 = CState m' fh i ((fh_ret pcv pcl)::s) fh_start true),
+     cstep cs1 ca cs2
 
-| cstep_push_p: forall m fh i s pcv pcl cv, 
-    fh @ pcv # Push cv ->
-    cstep (CState m fh i s (pcv,pcl) true) 
-          Silent (CState m fh i ((Vint cv,handlerTag):::s) (pcv+1,handlerTag) true)
+| cstep_push_p: forall m fh i s pcv pcl cv,
+    forall (INST: fh @ pcv # Push cv)
+           (CS1: cs1 = CState m fh i s (pcv,pcl) true)
+           (CA: ca = Silent)
+           (CS2: cs2 = CState m fh i ((Vint cv,handlerTag):::s) (pcv+1,handlerTag) true),
+    cstep cs1 ca cs2
 
 | cstep_pop: forall fh m i s rpcl pcv pcl rl xv xl,
    forall(INST: i @ pcv # Pop)
          (CHIT: cache_hit_mem m (opCodeToZ OpPop) (__ , __, __) pcl)
-         (CREAD: cache_hit_read_mem m rl rpcl),
-     cstep (CState m fh i ((xv,xl):::s) (pcv,pcl)   false)
-           Silent (CState m fh i (s) (pcv+1,rpcl) false)
+         (CREAD: cache_hit_read_mem m rl rpcl)
+         (CS1: cs1 = CState m fh i ((xv,xl):::s) (pcv,pcl)   false)
+         (CA: ca = Silent)
+         (CS2: cs2 = CState m fh i (s) (pcv+1,rpcl) false),
+     cstep cs1 ca cs2
 
 | cstep_pop_f: forall c' fh m i s pcv pcl xv xl m',
    forall(INST : i @ pcv # Pop)
          (CMISS: ~ cache_hit_mem m (opCodeToZ OpPop) (__,__,__) pcl)
          (CUPD : c' = build_cache (opCodeToZ OpPop) (__,__,__) pcl)
-         (CUPDGET : cupd m c' = Some m'),
-     cstep (CState m fh i ((xv,xl):::s) (pcv,pcl) false)  
-           Silent (CState m' fh i ((fh_ret pcv pcl)::(xv,xl):::s) fh_start true)
+         (CUPDGET : cupd m c' = Some m')
+         (CS1: cs1 = CState m fh i ((xv,xl):::s) (pcv,pcl) false)
+         (CA: ca = Silent)
+         (CS2: cs2 = CState m' fh i ((fh_ret pcv pcl)::(xv,xl):::s) fh_start true),
+     cstep cs1 ca cs2
 
-| cstep_pop_p: forall m fh i s pcv pcl xv xl, 
-    fh @ pcv # Pop ->
-    cstep (CState m fh i ((xv,xl):::s) (pcv,pcl) true) 
-          Silent (CState m fh i s (pcv+1,handlerTag) true)
+| cstep_pop_p: forall m fh i s pcv pcl xv xl,
+    forall (INST: fh @ pcv # Pop)
+           (CS1: cs1 = CState m fh i ((xv,xl):::s) (pcv,pcl) true)
+           (CA: ca = Silent)
+           (CS2: cs2 = CState m fh i s (pcv+1,handlerTag) true),
+    cstep cs1 ca cs2
 
-| cstep_push_cache_ptr_p: forall m fh i s pcv pcl, 
-    fh @ pcv # PushCachePtr ->
-    cstep (CState m fh i s (pcv,pcl) true) 
-          Silent (CState m fh i ((Vptr cblock 0,handlerTag):::s) (pcv+1,handlerTag) true)
+| cstep_push_cache_ptr_p: forall m fh i s pcv pcl,
+    forall (INST: fh @ pcv # PushCachePtr)
+           (CS1: cs1 = CState m fh i s (pcv,pcl) true)
+           (CA: ca = Silent)
+           (CS2: cs2 = CState m fh i ((Vptr cblock 0,handlerTag):::s) (pcv+1,handlerTag) true),
+    cstep cs1 ca cs2
 
 | cstep_alloc: forall fh m i s pcv pcl b size sizel xv xl m' rpcl rl,
-               forall (INST: i @ pcv # Alloc)
-                      (CHIT: cache_hit_mem m (opCodeToZ OpAlloc) (sizel, __, __) pcl)
-                      (CREAD: cache_hit_read_mem m rl rpcl)
-                      (ALLOC: c_alloc User size (xv,xl) m = Some (b,m')),
-                 cstep (CState m fh i (CData (Vint size, sizel)::CData (xv,xl)::s) (pcv,pcl) false)
-                       Silent
-                       (CState m' fh i (CData (Vptr b 0,rl)::s) (pcv+1,rpcl) false)
+    forall (INST: i @ pcv # Alloc)
+           (CHIT: cache_hit_mem m (opCodeToZ OpAlloc) (sizel, __, __) pcl)
+           (CREAD: cache_hit_read_mem m rl rpcl)
+           (ALLOC: c_alloc User size (xv,xl) m = Some (b,m'))
+           (CS1: cs1 = CState m fh i (CData (Vint size, sizel)::CData (xv,xl)::s) (pcv,pcl) false)
+           (CA: ca = Silent)
+           (CS2: cs2 = CState m' fh i (CData (Vptr b 0,rl)::s) (pcv+1,rpcl) false),
+      cstep cs1 ca cs2
 
 | cstep_alloc_f: forall c' fh m m' i s pcv pcl size sizel xv xl,
-                 forall (INST: i @ pcv # Alloc)
-                        (CMISS: ~ cache_hit_mem m (opCodeToZ OpAlloc) (sizel, __, __) pcl)
-                        (CUPD: c' = build_cache (opCodeToZ OpAlloc) (sizel, __, __) pcl)
-                        (CUPDGET: cupd m c' = Some m'),
-                   cstep (CState m fh i (CData (Vint size, sizel)::CData (xv,xl)::s) (pcv,pcl) false)
-                         Silent
-                         (CState m' fh i (fh_ret pcv pcl::CData (Vint size, sizel)::CData (xv,xl)::s) fh_start true)
+    forall (INST: i @ pcv # Alloc)
+           (CMISS: ~ cache_hit_mem m (opCodeToZ OpAlloc) (sizel, __, __) pcl)
+           (CUPD: c' = build_cache (opCodeToZ OpAlloc) (sizel, __, __) pcl)
+           (CUPDGET: cupd m c' = Some m')
+           (CS1: cs1 = CState m fh i (CData (Vint size, sizel)::CData (xv,xl)::s) (pcv,pcl) false)
+           (CA: ca = Silent)
+           (CS2: cs2 = CState m' fh i (fh_ret pcv pcl::CData (Vint size, sizel)::CData (xv,xl)::s) fh_start true),
+      cstep cs1 ca cs2
 
 | cstep_alloc_p: forall fh m m' i s pcv pcl b size sizel xv xl,
-                 forall (INST: fh @ pcv # Alloc)
-                        (ALLOC: c_alloc Kernel size (xv,xl) m = Some (b,m')),
-                   cstep (CState m fh i (CData (Vint size, sizel)::CData (xv,xl)::s) (pcv,pcl) true)
-                         Silent
-                         (CState m' fh i (CData (Vptr b 0,handlerTag)::s) (pcv+1,handlerTag) true)
+    forall (INST: fh @ pcv # Alloc)
+           (ALLOC: c_alloc Kernel size (xv,xl) m = Some (b,m'))
+           (CS1: cs1 = CState m fh i (CData (Vint size, sizel)::CData (xv,xl)::s) (pcv,pcl) true)
+           (CA: ca = Silent)
+           (CS2: cs2 = CState m' fh i (CData (Vptr b 0,handlerTag)::s) (pcv+1,handlerTag) true),
+      cstep cs1 ca cs2
 
 | cstep_load: forall fh m i s rpcl pcv pcl rl b ofs addrl xv xl,
    forall(INST: i @ pcv # Load)
          (CHIT: cache_hit_mem m (opCodeToZ OpLoad) (addrl, xl, __) pcl)
          (CREAD: cache_hit_read_mem m rl rpcl)
          (MREAD: load b ofs m = Some (xv,xl))
-         (PRIV: Mem.stamp b = User),
-     cstep (CState m fh i ((Vptr b ofs,addrl):::s) (pcv,pcl)   false)
-           Silent (CState m fh i ((xv,rl):::s) (pcv+1,rpcl) false)
+         (PRIV: Mem.stamp b = User)
+         (CS1: cs1 = CState m fh i ((Vptr b ofs,addrl):::s) (pcv,pcl)   false)
+         (CA: ca = Silent)
+         (CS2: cs2 = CState m fh i ((xv,rl):::s) (pcv+1,rpcl) false),
+     cstep cs1 ca cs2
 
 | cstep_load_f: forall c' fh m i s pcv pcl b ofs addrl xv xl m',
    forall(INST: i @ pcv # Load)
@@ -218,16 +266,20 @@ Inductive cstep : CS -> CEvent+τ -> CS -> Prop :=
          (MREAD: load b ofs m = Some (xv,xl))
          (CUPD : c' = build_cache (opCodeToZ OpLoad) (addrl,xl,__) pcl)
          (PRIV: Mem.stamp b = User)
-         (CUPDGET : cupd m c' = Some m'),
-     cstep (CState m fh i ((Vptr b ofs,addrl):::s) (pcv,pcl)   false)
-           Silent (CState m' fh i ((fh_ret pcv pcl)::(Vptr b ofs,addrl):::s) fh_start true)
+         (CUPDGET : cupd m c' = Some m')
+         (CS1: cs1 = CState m fh i ((Vptr b ofs,addrl):::s) (pcv,pcl)   false)
+         (CA: ca = Silent)
+         (CS2: cs2 = CState m' fh i ((fh_ret pcv pcl)::(Vptr b ofs,addrl):::s) fh_start true),
+     cstep cs1 ca cs2
 
 | cstep_load_p: forall m fh i s pcv pcl b ofs addrl x,
    forall (INST: fh @ pcv # Load)
           (READ: load b ofs m = Some x)
-          (PRIV: Mem.stamp b = Kernel),
-    cstep (CState m fh i ((Vptr b ofs,addrl):::s) (pcv,pcl) true) 
-          Silent (CState m fh i (x:::s) (pcv+1,handlerTag) true)
+          (PRIV: Mem.stamp b = Kernel)
+          (CS1: cs1 = CState m fh i ((Vptr b ofs,addrl):::s) (pcv,pcl) true)
+          (CA: ca = Silent)
+          (CS2: cs2 = CState m fh i (x:::s) (pcv+1,handlerTag) true),
+    cstep cs1 ca cs2
 
 | cstep_store: forall fh m m' i s rpcl pcv pcl rl b ofs addrl xv xl mv ml,
    forall(INST: i @ pcv # Store)
@@ -235,9 +287,11 @@ Inductive cstep : CS -> CEvent+τ -> CS -> Prop :=
          (CREAD: cache_hit_read_mem m rl rpcl)
          (MREAD: load b ofs m = Some (mv,ml))
          (MUPDT: store b ofs (xv,rl) m = Some m')
-         (PRIV: Mem.stamp b = User),
-     cstep (CState m fh i ((Vptr b ofs,addrl):::(xv,xl):::s) (pcv,pcl)   false)
-           Silent (CState m' fh i s (pcv+1,rpcl) false)
+         (PRIV: Mem.stamp b = User)
+         (CS1: cs1 = CState m fh i ((Vptr b ofs,addrl):::(xv,xl):::s) (pcv,pcl)   false)
+         (CA: ca = Silent)
+         (CS2: cs2 = CState m' fh i s (pcv+1,rpcl) false),
+     cstep cs1 ca cs2
 
 | cstep_store_f: forall c' fh m i s pcv pcl b ofs addrl xv xl mv ml m',
    forall(INST: i @ pcv # Store)
@@ -245,147 +299,185 @@ Inductive cstep : CS -> CEvent+τ -> CS -> Prop :=
          (MREAD: load b ofs m = Some (mv,ml))
          (CUPD : c' = build_cache (opCodeToZ OpStore) (addrl,xl,ml) pcl)
          (PRIV: Mem.stamp b = User)
-         (CUPDGET : cupd m c' = Some m'),
-     cstep (CState m fh i ((Vptr b ofs,addrl):::(xv,xl):::s) (pcv,pcl)   false)
-           Silent (CState m' fh i ((fh_ret pcv pcl)::(Vptr b ofs,addrl):::(xv,xl):::s) fh_start true)
+         (CUPDGET : cupd m c' = Some m')
+         (CS1: cs1 = CState m fh i ((Vptr b ofs,addrl):::(xv,xl):::s) (pcv,pcl)   false)
+         (CA: ca = Silent)
+         (CS2: cs2 = CState m' fh i ((fh_ret pcv pcl)::(Vptr b ofs,addrl):::(xv,xl):::s) fh_start true),
+     cstep cs1 ca cs2
 
-| cstep_store_p: forall m fh i s pcv pcl m' b ofs addrl x, 
+| cstep_store_p: forall m fh i s pcv pcl m' b ofs addrl x,
     forall (INST:fh @ pcv # Store)
            (UPD: store b ofs x m = Some m')
-           (PRIV: Mem.stamp b = Kernel),
-    cstep (CState m fh i ((Vptr b ofs,addrl)::: x :::s) (pcv,pcl) true)
-          Silent (CState m' fh i s (pcv+1,handlerTag) true)
+           (PRIV: Mem.stamp b = Kernel)
+           (CS1: cs1 = CState m fh i ((Vptr b ofs,addrl)::: x :::s) (pcv,pcl) true)
+           (CA: ca = Silent)
+           (CS2: cs2 = CState m' fh i s (pcv+1,handlerTag) true),
+    cstep cs1 ca cs2
 
 | cstep_jump: forall fh m i s rpcl pcv pcl rl cv cl,
    forall(INST: i @ pcv # Jump)
          (CHIT: cache_hit_mem m (opCodeToZ OpJump) (cl, __, __) pcl)
-         (CREAD: cache_hit_read_mem m rl rpcl),
-     cstep (CState m fh i ((Vint cv,cl):::s) (pcv,pcl)   false)
-           Silent (CState m fh i s (cv,rpcl) false)
+         (CREAD: cache_hit_read_mem m rl rpcl)
+         (CS1: cs1 = CState m fh i ((Vint cv,cl):::s) (pcv,pcl)   false)
+         (CA: ca = Silent)
+         (CS2: cs2 = CState m fh i s (cv,rpcl) false),
+     cstep cs1 ca cs2
 
 | cstep_jump_f: forall c' fh m i s pcv pcl cv cl m',
    forall(INST: i @ pcv # Jump)
          (CMISS: ~ cache_hit_mem m (opCodeToZ OpJump) (cl,__,__) pcl)
          (CUPD : c' = build_cache (opCodeToZ OpJump) (cl,__,__) pcl)
-         (CUPDGET : cupd m c' = Some m'),
-     cstep (CState m fh i ((cv,cl):::s) (pcv,pcl)   false)
-           Silent (CState m' fh i ((fh_ret pcv pcl)::(cv,cl):::s) fh_start true)
+         (CUPDGET : cupd m c' = Some m')
+         (CS1: cs1 = CState m fh i ((cv,cl):::s) (pcv,pcl)   false)
+         (CA: ca = Silent)
+         (CS2: cs2 = CState m' fh i ((fh_ret pcv pcl)::(cv,cl):::s) fh_start true),
+     cstep cs1 ca cs2
 
 | cstep_jump_p: forall m fh i s pcv pcl pcj pcjl,
-    forall (INST: fh @ pcv # Jump),
-    cstep (CState m fh i ((Vint pcj,pcjl):::s) (pcv,pcl) true) 
-          Silent (CState m fh i s (pcj,handlerTag) true)
+    forall (INST: fh @ pcv # Jump)
+           (CS1: cs1 = CState m fh i ((Vint pcj,pcjl):::s) (pcv,pcl) true)
+           (CA: ca = Silent)
+           (CS2: cs2 = CState m fh i s (pcj,handlerTag) true),
+    cstep cs1 ca cs2
 
 | cstep_bnz: forall fh m i s rpcl pcv pcl rl cv cl offv,
    forall(INST: i @ pcv # BranchNZ offv)
          (CHIT: cache_hit_mem m (opCodeToZ OpBranchNZ) (cl, __, __) pcl)
-         (CREAD: cache_hit_read_mem m rl rpcl),
-     cstep (CState m fh i ((Vint cv,cl):::s) (pcv,pcl)   false)
-           Silent (CState m fh i s (if cv =? 0 then pcv+1 else pcv+offv, rpcl) false)
+         (CREAD: cache_hit_read_mem m rl rpcl)
+         (CS1: cs1 = CState m fh i ((Vint cv,cl):::s) (pcv,pcl)   false)
+         (CA: ca = Silent)
+         (CS2: cs2 = CState m fh i s (if cv =? 0 then pcv+1 else pcv+offv, rpcl) false),
+     cstep cs1 ca cs2
 
 | cstep_bnz_f: forall c' fh m m' i s pcv pcl cv cl offv,
    forall(INST: i @ pcv # BranchNZ offv)
          (CMISS: ~ cache_hit_mem m (opCodeToZ OpBranchNZ) (cl,__,__) pcl)
          (CUPD : c' = build_cache (opCodeToZ OpBranchNZ) (cl,__,__) pcl)
-         (CUPDGET: cupd m c' = Some m'),
-     cstep (CState m fh i ((Vint cv,cl):::s) (pcv,pcl)   false)
-           Silent (CState m' fh i ((fh_ret pcv pcl)::(Vint cv,cl):::s) fh_start true)
+         (CUPDGET: cupd m c' = Some m')
+         (CS1: cs1 = CState m fh i ((Vint cv,cl):::s) (pcv,pcl)   false)
+         (CA: ca = Silent)
+         (CS2: cs2 = CState m' fh i ((fh_ret pcv pcl)::(Vint cv,cl):::s) fh_start true),
+     cstep cs1 ca cs2
 
 | cstep_branchnz_p: forall m fh i s pcv pcl offv av al,
-    forall (INST: fh @ pcv # BranchNZ offv),
-    cstep (CState m fh i ((Vint av,al):::s) (pcv,pcl) true) 
-          Silent (CState m fh i s (if av =? 0 then pcv+1 else pcv+offv, handlerTag) true)
+    forall (INST: fh @ pcv # BranchNZ offv)
+           (CS1: cs1 = CState m fh i ((Vint av,al):::s) (pcv,pcl) true)
+           (CA: ca = Silent)
+           (CS2: cs2 = CState m fh i s (if av =? 0 then pcv+1 else pcv+offv, handlerTag) true),
+    cstep cs1 ca cs2
 
 | cstep_call: forall fh m i s rpcl pcv pcl rl pcc pccl a r args,
    forall(INST: i @ pcv # Call a r)
-         (ARGSA: length args = a) 
+         (ARGSA: length args = a)
          (ARGS: forall a, In a args -> exists d, a = CData d)
          (CHIT: cache_hit_mem m (opCodeToZ OpCall) (pccl, __, __) pcl)
-         (CREAD: cache_hit_read_mem m rl rpcl),
-     cstep (CState m fh i ((Vint pcc,pccl):::args++s) (pcv,pcl)   false)
-           Silent (CState m fh i (args++(((CRet (pcv+1, rl)) r false)::s)) (pcc,rpcl) false)
+         (CREAD: cache_hit_read_mem m rl rpcl)
+         (CS1: cs1 = CState m fh i ((Vint pcc,pccl):::args++s) (pcv,pcl)   false)
+         (CA: ca = Silent)
+         (CS2: cs2 = CState m fh i (args++(((CRet (pcv+1, rl)) r false)::s)) (pcc,rpcl) false),
+     cstep cs1 ca cs2
 
 | cstep_call_f: forall c' fh m i s pcv pcl pcc pccl a r args m',
    forall(INST: i @ pcv # Call a r)
-         (ARGSA: length args = a) 
+         (ARGSA: length args = a)
          (ARGS: forall a, In a args -> exists d, a = CData d)
          (CMISS: ~ cache_hit_mem m (opCodeToZ OpCall) (pccl, __, __) pcl)
          (CUPD : c' = build_cache (opCodeToZ OpCall) (pccl,__,__) pcl)
-         (CUPDGET : cupd m c' = Some m'),
-     cstep (CState m fh i ((pcc,pccl):::args++s) (pcv,pcl)   false)
-           Silent (CState m' fh i ((fh_ret pcv pcl)::(pcc,pccl):::args++s) fh_start true)
+         (CUPDGET : cupd m c' = Some m')
+         (CS1: cs1 = CState m fh i ((pcc,pccl):::args++s) (pcv,pcl)   false)
+         (CA: ca = Silent)
+         (CS2: cs2 = CState m' fh i ((fh_ret pcv pcl)::(pcc,pccl):::args++s) fh_start true),
+     cstep cs1 ca cs2
 
 | cstep_call_p: forall m fh i s pcv pcl a r args pcc pccl,
     forall (INST: fh @ pcv # Call a r)
            (ARGSA: length args = a)
-           (ARGS: forall a, In a args -> exists d, a = CData d),
-    cstep (CState m fh i ((Vint pcc,pccl):::args++s) (pcv,pcl) true) 
-          Silent (CState m fh i (args++(CRet (pcv+1, pcl) r true)::s) (pcc, handlerTag) true)
+           (ARGS: forall a, In a args -> exists d, a = CData d)
+           (CS1: cs1 = CState m fh i ((Vint pcc,pccl):::args++s) (pcv,pcl) true)
+           (CA: ca = Silent)
+           (CS2: cs2 = CState m fh i (args++(CRet (pcv+1, pcl) r true)::s) (pcc, handlerTag) true),
+    cstep cs1 ca cs2
 
 | cstep_ret: forall fh m i s s' pcv pcl rl rpcl pcret pcretl,
    forall(INST: i @ pcv # Ret)
          (CHIT: cache_hit_mem m (opCodeToZ OpRet) (pcretl, __, __) pcl)
-         (POP:  c_pop_to_return s ((CRet (pcret,pcretl) false false)::s')) 
+         (POP:  c_pop_to_return s ((CRet (pcret,pcretl) false false)::s'))
                 (*DD: should only return to user mode *)
-         (CREAD: cache_hit_read_mem m rl rpcl),
-     cstep (CState m fh i s  (pcv,pcl) false)
-           Silent (CState m fh i s' (pcret, rpcl) false)
+         (CREAD: cache_hit_read_mem m rl rpcl)
+         (CS1: cs1 = CState m fh i s  (pcv,pcl) false)
+         (CA: ca = Silent)
+         (CS2: cs2 = CState m fh i s' (pcret, rpcl) false),
+     cstep cs1 ca cs2
 
 | cstep_ret_f: forall c' fh m i s' s pcv pcl pret pcret pcretl m',
    forall(INST: i @ pcv # Ret)
          (CMISS: ~ cache_hit_mem m (opCodeToZ OpRet) (pcretl, __, __) pcl)
-         (POP:  c_pop_to_return s ((CRet (pcret,pcretl) false pret)::s')) 
+         (POP:  c_pop_to_return s ((CRet (pcret,pcretl) false pret)::s'))
          (*DD: same thing, but we need not to constraint the return
                mode here, actually. *)
          (CUPD : c' = build_cache (opCodeToZ OpRet) (pcretl,__,__) pcl)
-         (CUPDGET : cupd m c' = Some m'),
-     cstep (CState m fh i s  (pcv,pcl) false)
-           Silent (CState m' fh i ((fh_ret pcv pcl)::s) fh_start true)
+         (CUPDGET : cupd m c' = Some m')
+         (CS1: cs1 = CState m fh i s  (pcv,pcl) false)
+         (CA: ca = Silent)
+         (CS2: cs2 = CState m' fh i ((fh_ret pcv pcl)::s) fh_start true),
+     cstep cs1 ca cs2
 
-| cstep_ret_p: forall m fh i s pcv pcl  pcret pcretl s' pret, 
+| cstep_ret_p: forall m fh i s pcv pcl  pcret pcretl s' pret,
     forall (INST: fh @ pcv # Ret) (* can either return to user/priv mode *)
-           (POP: c_pop_to_return s ((CRet (pcret,pcretl) false pret)::s')),
-    cstep (CState m fh i s  (pcv,pcl) true) 
-          Silent (CState m fh i s' (pcret,pcretl) pret)
+           (POP: c_pop_to_return s ((CRet (pcret,pcretl) false pret)::s'))
+           (CS1: cs1 = CState m fh i s  (pcv,pcl) true)
+           (CA: ca = Silent)
+           (CS2: cs2 = CState m fh i s' (pcret,pcretl) pret),
+    cstep cs1 ca cs2
 
 | cstep_vret: forall fh m i s s' pcv pcl rl rpcl resv resl pcret pcretl,
    forall(INST: i @ pcv # VRet)
          (CHIT: cache_hit_mem m (opCodeToZ OpVRet) (resl, pcretl, __) pcl)
-         (POP:  c_pop_to_return s ((CRet (pcret,pcretl) true false)::s')) 
+         (POP:  c_pop_to_return s ((CRet (pcret,pcretl) true false)::s'))
                 (*DD: should only return to user mode *)
-         (CREAD: cache_hit_read_mem m rl rpcl),
-     cstep (CState m fh i ((resv,resl):::s)  (pcv,pcl) false)
-           Silent (CState m fh i ((resv,rl):::s') (pcret,rpcl) false)
+         (CREAD: cache_hit_read_mem m rl rpcl)
+         (CS1: cs1 = CState m fh i ((resv,resl):::s)  (pcv,pcl) false)
+         (CA: ca = Silent)
+         (CS2: cs2 = CState m fh i ((resv,rl):::s') (pcret,rpcl) false),
+     cstep cs1 ca cs2
 
 | cstep_vret_f: forall c' fh m i s' s pcv pcl resv resl pcret pcretl m',
    forall(INST: i @ pcv # VRet)
          (CMISS: ~ cache_hit_mem m (opCodeToZ OpVRet) (resl, pcretl, __) pcl)
          (POP:  c_pop_to_return s ((CRet (pcret,pcretl) true false)::s')) (*DD: same thing *)
          (CUPD : c' = build_cache (opCodeToZ OpVRet) (resl,pcretl,__) pcl)
-         (CUPDGET : cupd m c' = Some m'),
-     cstep (CState m fh i ((resv,resl):::s)  (pcv,pcl) false)
-           Silent (CState m' fh i ((fh_ret pcv pcl)::(resv,resl):::s) fh_start true)
+         (CUPDGET : cupd m c' = Some m')
+         (CS1: cs1 = CState m fh i ((resv,resl):::s)  (pcv,pcl) false)
+         (CA: ca = Silent)
+         (CS2: cs2 = CState m' fh i ((fh_ret pcv pcl)::(resv,resl):::s) fh_start true),
+     cstep cs1 ca cs2
 
-| cstep_vret_p: forall m fh i s pcv pcl s' pcret pcretl resv resl pret, 
+| cstep_vret_p: forall m fh i s pcv pcl s' pcret pcretl resv resl pret,
     forall (INST: fh @ pcv # VRet) (* cannot vreturn to user mode *)
-           (POP: c_pop_to_return s ((CRet (pcret,pcretl) true pret)::s')),
-    cstep (CState m fh i ((resv,resl):::s) (pcv,pcl) true) 
-          Silent (CState m fh i ((resv,resl):::s') (pcret, pcretl) pret)
+           (POP: c_pop_to_return s ((CRet (pcret,pcretl) true pret)::s'))
+           (CS1: cs1 = CState m fh i ((resv,resl):::s) (pcv,pcl) true)
+           (CA: ca = Silent)
+           (CS2: cs2 = CState m fh i ((resv,resl):::s') (pcret, pcretl) pret),
+    cstep cs1 ca cs2
 
 | cstep_out: forall fh m i s rpcl pcv pcl rl cv cl,
    forall(INST: i @ pcv # Output)
          (CHIT: cache_hit_mem m (opCodeToZ OpOutput) (cl, __, __) pcl)
-         (CREAD: cache_hit_read_mem m rl rpcl),
-     cstep (CState m fh i ((Vint cv,cl):::s) (pcv,pcl)   false)
-           (E (CEInt (cv,rl) m)) (CState m fh i s (pcv+1,rpcl) false)
+         (CREAD: cache_hit_read_mem m rl rpcl)
+         (CS1: cs1 = CState m fh i ((Vint cv,cl):::s) (pcv,pcl)   false)
+         (CA: ca = (E (CEInt (cv,rl) m)))
+         (CS2: cs2 = CState m fh i s (pcv+1,rpcl) false),
+     cstep cs1 ca cs2
 
 | cstep_out_f: forall c' fh m i s pcv pcl cv cl m',
    forall(INST: i @ pcv # Output)
          (CMISS: ~ cache_hit_mem m (opCodeToZ OpOutput) (cl,__,__) pcl)
          (CUPD : c' = build_cache (opCodeToZ OpOutput) (cl,__,__) pcl)
-         (CUPDGET : cupd m c' = Some m'),
-     cstep (CState m fh i ((Vint cv,cl):::s) (pcv,pcl)   false)
-           Silent (CState m' fh i ((fh_ret pcv pcl)::(Vint cv,cl):::s) fh_start true).
+         (CUPDGET : cupd m c' = Some m')
+         (CS1: cs1 = CState m fh i ((Vint cv,cl):::s) (pcv,pcl)   false)
+         (CA: ca = Silent)
+         (CS2: cs2 = CState m' fh i ((fh_ret pcv pcl)::(Vint cv,cl):::s) fh_start true),
+     cstep cs1 ca cs2.
 
 Definition concrete_machine (faultHandler: list Instr) : semantics :=
   {| state := CS ;
